$$-\frac{1}{8}\int -8\cos-8x \, dx = \begin{array}
|t = -8x \\
dt = -8dx
\end{array}
=-\frac{1}{8}\int \cos t \, dt = -\frac{1}{8}\sin-8x + c 
$$

###### !!!!!!!!!!!!!!!!!!!!!!!!!!!!!!!!!!!!!!!!!!!!!!!!!!!!!!!!!!!!!!!!!



$$
\int (-x^{2}+4x-7)e^\frac{x}{2} \, dx = \begin{array}
|u = -x^{2}+4x-7 & u'=-2x+4 \\
v'=e^\frac{x}{2} & v=2e^\frac{x}{2}
\end{array}
$$
$$
= (-x^{2}+4x-7)\left( 2e^\frac{x}{2} \right)-\int (-2x+4)2e^\frac{x}{2} \, dx =\begin{array}
|u = -2x+4 & u'=-2 \\
v'=2e^\frac{x}{2} & v=4e^\frac{x}{2}
\end{array}
$$
$$
(-x^{2}+4x-7)\left( 2e^\frac{x}{2} \right) - \left( (-2x+4)\left( 4e^\frac{x}{2} \right) - \int -8e^\frac{x}{2} \, dx  \right)
$$
$$
(-x^{2}+4x-7)\left( 2e^\frac{x}{2} \right) - \left( (-2x+4)\left( 4e^\frac{x}{2} \right) +16e^\frac{x}{2}\right) = (-x^{2}+4x-7)\left( 2e^\frac{x}{2} \right) - \left( 2e^\frac{x}{2} \right)(-4x+16) = \left(e^\frac{x}{2} \right)(-2x^2+16x-46)+c
$$
